Examples/Reverse32Bit.lean
@@ -18,7 +18,7 @@ def reverse_32bit : {chunks : Nat} → BitVec (32 * chunks) → BitVec (32 * chu
   | chunks + 1, bits =>
       bitmatch bits with
       | <<x : 32, rest : (32 * chunks)>> => <<(reverse_32bit rest), x : 32>>
-
+-- #print reverse_32bit
 def example51Input : BitVec 96 :=
   <<0x11111111:32, 0x22222222:32, 0x33333333:32>>
 
@@ -29,6 +29,6 @@ def example51Reversed : BitVec 96 :=
   reverse_32bit (chunks := 3) example51Input
 
 example : example51Reversed = example51Expected := by
-  rfl
+  native_decide
 
 end LeanBitsyntax
